src/ext_traversal/ExtSimTraversal.v
@@ -12,6 +12,7 @@ From imm Require Import AuxDef.
 Require Import TraversalConfig.
 Require Import TraversalConfigAlt.
 Require Import Traversal.
+Require Import ExtTraversalConfig.
 Require Import ExtTraversal.
 Require Import AuxRel AuxRel2.
 
