src/ext_traversal/ExtSimTraversalProperties.v
@@ -1,6 +1,6 @@
 From hahn Require Import Hahn.
 From imm Require Import Events Execution imm_s AuxDef.
-Require Import ExtTraversal.
+Require Import ExtTraversalConfig.
 Require Import ExtSimTraversal.
 
 Set Implicit Arguments.
