src/ext_traversal/ExtTraversalConfig.v
@@ -1,0 +1,139 @@
+Require Import Setoid.
+From hahn Require Import Hahn.
+From imm Require Import AuxDef Events Execution Execution_eco
+     imm_bob imm_s_ppo imm_s imm_s_hb CombRelations.
+Require Import TraversalConfig Traversal.
+Require Import AuxRel AuxRel2.
+Require Export ExtTravRelations.
+Require Import TraversalProperties.
+Require Import ImmProperties.
+
+Set Implicit Arguments.
+
+Section ExtTraversalConfig.
+Variable G : execution.
+Variable sc : relation actid.
+
+Notation "'acts'" := G.(acts).
+Notation "'sb'" := G.(sb).
+Notation "'rmw'" := G.(rmw).
+Notation "'data'" := G.(data).
+Notation "'addr'" := G.(addr).
+Notation "'ctrl'" := G.(ctrl).
+Notation "'rmw_dep'" := G.(rmw_dep).
+Notation "'rf'" := G.(rf).
+Notation "'co'" := G.(co).
+Notation "'coe'" := G.(coe).
+Notation "'fr'" := G.(fr).
+
+Notation "'eco'" := G.(eco).
+
+Notation "'bob'" := G.(bob).
+Notation "'fwbob'" := G.(fwbob).
+Notation "'ppo'" := G.(ppo).
+Notation "'rppo'" := G.(rppo).
+Notation "'fre'" := G.(fre).
+Notation "'rfi'" := G.(rfi).
+Notation "'rfe'" := G.(rfe).
+Notation "'deps'" := G.(deps).
+Notation "'detour'" := G.(detour).
+Notation "'release'" := G.(release).
+Notation "'sw'" := G.(sw).
+Notation "'hb'" := G.(hb).
+
+Notation "'urr'" := (urr G sc).
+Notation "'c_acq'" := (c_acq G sc).
+Notation "'c_cur'" := (c_cur G sc).
+Notation "'c_rel'" := (c_rel G sc).
+Notation "'t_acq'" := (t_acq G sc).
+Notation "'t_cur'" := (t_cur G sc).
+Notation "'t_rel'" := (t_rel G sc).
+Notation "'S_tm'" := G.(S_tm).
+Notation "'S_tmr'" := G.(S_tmr).
+Notation "'msg_rel'" := (msg_rel G sc).
+
+Notation "'lab'" := G.(lab).
+Notation "'loc'" := (loc lab).
+Notation "'val'" := (val lab).
+Notation "'mod'" := (Events.mod lab).
+Notation "'same_loc'" := (same_loc lab).
+
+Notation "'E'" := G.(acts_set).
+Notation "'R'" := (fun x => is_true (is_r lab x)).
+Notation "'W'" := (fun x => is_true (is_w lab x)).
+Notation "'F'" := (fun x => is_true (is_f lab x)).
+Notation "'RW'" := (R ∪₁ W).
+Notation "'FR'" := (F ∪₁ R).
+Notation "'FW'" := (F ∪₁ W).
+Notation "'R_ex'" := (fun a => is_true (R_ex lab a)).
+Notation "'W_ex'" := (W_ex G).
+Notation "'W_ex_acq'" := (W_ex ∩₁ (fun a => is_true (is_xacq lab a))).
+
+Notation "'Init'" := (fun a => is_true (is_init a)).
+Notation "'Loc_' l" := (fun x => loc x = Some l) (at level 1).
+Notation "'Tid_' t" := (fun x => tid x = t) (at level 1).
+Notation "'W_' l" := (W ∩₁ Loc_ l) (at level 1).
+
+Notation "'Pln'" := (fun x => is_true (is_only_pln lab x)).
+Notation "'Rlx'" := (fun x => is_true (is_rlx lab x)).
+Notation "'Rel'" := (fun x => is_true (is_rel lab x)).
+Notation "'Acq'" := (fun x => is_true (is_acq lab x)).
+Notation "'Acqrel'" := (fun x => is_true (is_acqrel lab x)).
+Notation "'Sc'" := (fun x => is_true (is_sc lab x)).
+Notation "'Acq/Rel'" := (fun a => is_true (is_ra lab a)).
+
+(******************************************************************************)
+(** **   *)
+(******************************************************************************)
+
+Record ext_trav_config :=
+  mkETC { etc_TC : trav_config; reserved : actid -> Prop; }.
+
+Definition eissued  T := issued  (etc_TC T).
+Definition ecovered T := covered (etc_TC T).
+
+Definition dom_sb_S_rfrmw T rrf P :=
+  dom_rel (⦗W_ex⦘ ⨾ sb ⨾ ⦗reserved T⦘) ∩₁ codom_rel (⦗P⦘ ⨾ rrf ⨾ rmw) ∩₁ codom_rel (rmw ∩ ctrl).
+
+Record etc_coherent (T : ext_trav_config) :=
+  mkETCC {
+      etc_tccoh  : tc_coherent G sc (etc_TC T);
+
+      etc_S_in_E : reserved T ⊆₁ E;
+      etc_I_in_S : eissued T ⊆₁ reserved T;
+      etc_S_I_in_W_ex : reserved T \₁ eissued T ⊆₁ W_ex;
+
+      etc_F_sb_S : dom_rel (⦗F∩₁Acq/Rel⦘ ⨾ sb ⨾ ⦗reserved T⦘) ⊆₁ ecovered T ;
+      etc_dr_R_acq_I :
+        dom_rel ((detour ∪ rfe) ⨾ ⦗R∩₁Acq⦘ ⨾ sb ⨾ ⦗reserved T⦘) ⊆₁ eissued T ;
+      etc_W_ex_sb_I : dom_rel (⦗W_ex_acq⦘ ⨾ sb ⨾ ⦗reserved T⦘) ⊆₁ eissued T ;
+      
+      etc_sb_S :
+        dom_sb_S_rfrmw T rf (eissued T) ⊆₁ reserved T;
+
+      etc_rppo_S :
+        dom_rel ((detour ∪ rfe) ⨾ (data ∪ rfi)＊ ⨾ rppo ⨾ ⦗ reserved T ⦘) ⊆₁ eissued T;
+
+      etc_S_W_ex_rfrmw_I : reserved T ∩₁ W_ex ⊆₁ codom_rel (⦗eissued T⦘ ⨾ rf ⨾ rmw);
+    }.
+
+Section Props.
+
+Variable WF : Wf G.
+Variable T : ext_trav_config.
+Variable ETCCOH : etc_coherent T.
+
+Lemma eissuedW : eissued T ⊆₁ W.
+Proof using ETCCOH. unfold eissued. eapply issuedW. apply ETCCOH. Qed.
+
+Lemma reservedW : reserved T ⊆₁ W.
+Proof using WF ETCCOH.
+  arewrite (reserved T ⊆₁ reserved T \₁ eissued T ∪₁ reserved T ∩₁ eissued T).
+  2: { rewrite eissuedW at 2; auto. rewrite etc_S_I_in_W_ex; auto.
+       rewrite W_ex_in_W; auto. basic_solver. }
+  unfolder. ins.
+  destruct (classic (eissued T x)); eauto.
+Qed.
+
+End Props.
+End ExtTraversalConfig.
