src/ext_traversal/ExtTraversalCounting.v
@@ -6,7 +6,7 @@ From imm Require Import Events Execution imm_s.
 Require Import AuxRel2.
 Require Import TraversalConfig.
 Require Import Traversal.
-Require Import ExtTraversal.
+Require Import ExtTraversalConfig.
 Require Import ExtSimTraversal.
 Require Import ExtSimTraversalProperties.
 
