src/ext_traversal/ExtTraversalProperties.v
@@ -4,7 +4,7 @@ From imm Require Import Events Execution Execution_eco
      imm_bob imm_s_ppo imm_s imm_s_hb CombRelations AuxDef.
 Require Import AuxRel AuxRel2.
 Require Import TraversalConfig Traversal.
-Require Import ExtTraversal.
+Require Import ExtTraversalConfig.
 Require Import ImmProperties.
 
 Set Implicit Arguments.
